---
title: "Class 13: Thinking, Fast and Slow"
author: "Taylor Arnold"
output: html_notebook
---


```{r setup, include=FALSE}
knitr::opts_chunk$set(eval = TRUE)
knitr::opts_chunk$set(fig.path = "../assets/2017-10-10-class13/")
```

```{r, message = FALSE}
library(readr)
library(ggplot2)
library(dplyr)
library(methods)
```


## Stochastic Gradient Descent

$$ \left( w^{(0)} - \eta \cdot \nabla_w f \right) \, \rightarrow \, w^{(1)} $$

$$ \begin{align} f(w) &= \sum_i (\widehat{y}_i(w) - y_i)^2 \\
        &= \sum_i f_i(w) \\
        \nabla_w f &= \sum_i \nabla_w f_i
    \end{align}$$

$$
\begin{align}
\left( w^{(0)} - (\eta / n) \cdot \nabla_{w^{(0)}} f_1 \right) \, &\rightarrow \, w^{(1)} \\
\left( w^{(1)} - (\eta / n) \cdot \nabla_{w^{(0)}} f_2 \right) \, &\rightarrow \, w^{(2)} \\
&\vdots \\
\left( w^{(n-1)} - (\eta / n) \cdot \nabla_{w^{(0)}} f_n \right) \, &\rightarrow \, w^{(n)} \\
\end{align}
$$

The $w^{(n)}$ here is exactly equivalent to the $w^{(1)}$ from before.

$$
\begin{align}
\left( w^{(0)} - \eta' \cdot \nabla_{w^{(0)}} f_1 \right) \, &\rightarrow \, w^{(1)} \\
\left( w^{(1)} - \eta' \cdot \nabla_{w^{(1)}} f_2 \right) \, &\rightarrow \, w^{(2)} \\
&\vdots \\
\left( w^{(n-1)} - \eta' \cdot \nabla_{w^{(n)}} f_n \right) \, &\rightarrow \, w^{(n)} \\
\end{align}
$$




